Otway-Rees: progress - proved epred for event_forward_key
Apparently, it was necessary to extend a module in DYStar, SecrecyLabels, with
another Lemma readers_is_injective_2 which states the same as the first pred.
but for two readers instead of just one.

otway-rees-fixed/OYRS.Messages.fst
@@ -65,6 +65,8 @@ let parse_encval #i #l (sev:ser_encval i l) =
   )
   | (|t,_|) -> Error ("invalid tag: " ^ t)
 
+let parse_encval_lemma #i #l sev = ()
+
 let parse_serialize_encval_lemma i ev l = ()
 
 let parsed_encval_is_valid_lemma #i #l sev = ()
