otway-rees-fixed/OYRS.Protocol.fst
@@ -266,7 +266,9 @@ let server_send_msg_3 srv msg2_idx =
       | Error e -> error ("srv_send_m3: decryption of initiator part failed: " ^ e)
   )
   | _ -> error "srv_send_m3: wrong message\n"
+#pop-options
 
+#push-options "--z3rlimit 500"
 let responder_send_msg_4 b msg3_idx b_si =
   // get responder session
   let now = global_timestamp () in
@@ -298,48 +300,73 @@ let responder_send_msg_4 b msg3_idx b_si =
               if n_b <> n_b' then error "r_send_m4: responder nonce in message does not match with the stored nonce\n"
               else if a <> a' then error "r_send_m4: stored initiator does not match with initiator in part encrypted for responder\n"
               else
-                // trigger event 'forward key'
-                // k_bs readers corrupted ?
-                publishable_readers_implies_corruption #now [P b; P srv];
-                // readers corrupted or aead pred holds
+                // k_bs publishable or aead_pred holds
                 assert(is_publishable oyrs_global_usage now k_bs
                   \/ aead_pred oyrs_usage_preds now "sk_r_srv" k_bs ser_ev_b ad);
+                // if k_bs publishable, k_bs readers flow to public
+                assert(is_publishable oyrs_global_usage now k_bs
+                  ==> can_flow now (get_label oyrs_key_usages k_bs) public);
+                // k_bs readable by responder and server
+                assert(is_labeled oyrs_global_usage now k_bs (readers [P b; P srv]));
+                // k_bs readers flow to public -> k_bs readers corrupted
+                publishable_readers_implies_corruption #now [P b; P srv];
+                // k_bs readers corrupted or aead_pred holds
+                includes_corrupt_2_lemma now (P b) (P srv);
+                assert((corrupt_id now (P b)) \/ (corrupt_id now (P srv))
+                  \/ aead_pred oyrs_usage_preds now "sk_r_srv" k_bs ser_ev_b ad);
 
-                // if aead pred holds, can aead encrypt from usage preds holds for earlier ts
-                assert(aead_pred oyrs_usage_preds now "sk_r_srv" k_bs ser_ev_b ad
-                  ==> (exists i. later_than now i /\ oyrs_usage_preds.can_aead_encrypt i "sk_r_srv" k_bs ser_ev_b ad));
+                // if aead_pred holds, oyrs_aead_pred holds for some timestamp before now
                 assert(aead_pred oyrs_usage_preds now "sk_r_srv" k_bs ser_ev_b ad
                   ==> (exists i. later_than now i /\ oyrs_aead_pred i "sk_r_srv" k_bs ser_ev_b ad));
-                // plug in definition of can aead encrypt from usage preds
+                // k_bs readers corrupted or oyrs_aead_pred holds for some timestamp before now
+                assert((corrupt_id now (P b)) \/ (corrupt_id now (P srv))
+                  \/ (exists i. later_than now i /\ oyrs_aead_pred i "sk_r_srv" k_bs ser_ev_b ad));
+
+                // plug in definition of oyrs_aead_pred
                 assert(exists i. (later_than now i /\ oyrs_aead_pred i "sk_r_srv" k_bs ser_ev_b ad)
                   ==> (forall (t:string{CryptoLib.bytes_to_string ad = Success t}). can_aead_encrypt i "sk_r_srv" k_bs (|t,ser_ev_b|) ad));
-                assert(aead_pred oyrs_usage_preds now "sk_r_srv" k_bs ser_ev_b ad
-                  ==> (exists i. forall (t:string{CryptoLib.bytes_to_string ad = Success t}). later_than now i /\ can_aead_encrypt i "sk_r_srv" k_bs (|t,ser_ev_b|) ad)); // implication transitive step 1
+                assert((corrupt_id now (P b)) \/ (corrupt_id now (P srv))
+                  \/ (exists i. forall (t:string{CryptoLib.bytes_to_string ad = Success t}). later_than now i /\ can_aead_encrypt i "sk_r_srv" k_bs (|t,ser_ev_b|) ad));
 
-                assert(tag_ev_b = "ev3_r");
-
-                // all strings t -> associated tag
+                // tag_ev_b is concrete value for t
+                assert(CryptoLib.bytes_to_string ad = Success tag_ev_b);
+                // can_aead_encrypt holds for all t -> holds for concrete t
                 can_aead_encrypt_encval_lemma now tag_ev_b (get_label oyrs_key_usages k_bs) "sk_r_srv" k_bs ser_ev_b ad;
-                assert(exists i. forall (t:string{CryptoLib.bytes_to_string ad = Success t}). (later_than now i /\ can_aead_encrypt i "sk_r_srv" k_bs (|t,ser_ev_b|) ad)
-                  ==> can_aead_encrypt i "sk_r_srv" k_bs (|tag_ev_b,ser_ev_b|) ad);
-                assert(aead_pred oyrs_usage_preds now "sk_r_srv" k_bs ser_ev_b ad
-                  ==> (exists i. later_than now i /\ can_aead_encrypt i "sk_r_srv" k_bs (|tag_ev_b,ser_ev_b|) ad)); // implication transitive step 2
-                assert(exists i. (later_than now i /\ can_aead_encrypt i "sk_r_srv" k_bs (|tag_ev_b,ser_ev_b|) ad)
-                  ==> (exists c n_a. did_event_occur_before i srv (event_send_key c a b srv n_a n_b k_ab)));
-                assert(aead_pred oyrs_usage_preds now "sk_r_srv" k_bs ser_ev_b ad
-                  ==> (exists i c n_a. later_than now i /\ did_event_occur_before i srv (event_send_key c a b srv n_a n_b k_ab))); // implication transitive step 3
-                assert(exists i c n_a. later_than now i /\ did_event_occur_before i srv (event_send_key c a b srv n_a n_b k_ab)
-                  ==> did_event_occur_before now srv (event_send_key c a b srv n_a n_b k_ab));
+                // if can_aead_encrypt holds for all t, it holds for tag_ev_b
+                assert((exists i. forall (t:string{CryptoLib.bytes_to_string ad = Success t}). later_than now i /\ can_aead_encrypt i "sk_r_srv" k_bs (|t,ser_ev_b|) ad)
+                  ==> (exists i. later_than now i /\ can_aead_encrypt i "sk_r_srv" k_bs (|tag_ev_b,ser_ev_b|) ad));
+                // k_bs readers corrupted or can_aead_encrypt holds for tag_ev_b
+                assert((corrupt_id now (P b)) \/ (corrupt_id now (P srv))
+                  \/ (exists i. later_than now i /\ can_aead_encrypt i "sk_r_srv" k_bs (|tag_ev_b,ser_ev_b|) ad));
 
-                // implication transitive
-                assert(aead_pred oyrs_usage_preds now "sk_r_srv" k_bs ser_ev_b ad
+                // prepare F* for rest of proof
+                (*** NOTE: THIS LEMMA IS NOT PART OF THE PUBLIC DY* VERSION ***)
+                readers_is_injective_2 b srv;
+                parse_encval_lemma #now #(get_label oyrs_key_usages k_bs) (|tag_ev_b,ser_ev_b|);
+                assert(get_label oyrs_key_usages k_bs == (readers [P b; P srv])
+                  /\ _parse_encval (|tag_ev_b,ser_ev_b|) == Success (EncMsg3_R n_b a k_ab));
+                assert((corrupt_id now (P b)) \/ (corrupt_id now (P srv))
+                  \/ (exists i. later_than now i /\ get_label oyrs_key_usages k_bs == (readers [P b; P srv]) /\ (exists c n_a. did_event_occur_before i srv (event_send_key c a b srv n_a n_b k_ab))));
+
+                // if can_aead_encrypt holds for tag_ev_b, event_send_key occured before some timestamp before now
+                assert((exists i. later_than now i /\ can_aead_encrypt i "sk_r_srv" k_bs (|tag_ev_b,ser_ev_b|) ad)
+                  ==> (exists i. later_than now i /\ (exists c n_a. did_event_occur_before i srv (event_send_key c a b srv n_a n_b k_ab))));
+                // k_bs readers corrupted or event_send_key occured before some timestamp before now
+                assert((corrupt_id now (P b)) \/ (corrupt_id now (P srv))
+                  \/ (exists i. later_than now i /\ (exists c n_a. did_event_occur_before i srv (event_send_key c a b srv n_a n_b k_ab))));
+
+                // if event_send_key occured before some timestamp before now, it occured before now (AHOI, captain obvious)
+                assert((exists i c n_a. later_than now i /\ did_event_occur_before i srv (event_send_key c a b srv n_a n_b k_ab))
                   ==> (exists c n_a. did_event_occur_before now srv (event_send_key c a b srv n_a n_b k_ab)));
-                // substitute aead pred with implication
-                assert(is_publishable oyrs_global_usage now k_bs \/ (exists c n_a. did_event_occur_before now srv (event_send_key c a b srv n_a n_b k_ab)));
-                assert((exists c n_a. did_event_occur_before now srv (event_send_key c a b srv n_a n_b k_ab)) \/ (corrupt_id now (P srv)) \/ (corrupt_id now (P b)));
+                // k_bs readers corrupted or event_send_key occured before now
+                assert((corrupt_id now (P b)) \/ (corrupt_id now (P srv))
+                  \/ (exists c n_a. did_event_occur_before now srv (event_send_key c a b srv n_a n_b k_ab)));
+
+                // trigger event 'forward key'
                 let prev = now in
                 let event = event_forward_key c a b srv k_ab in
                 trigger_event #oyrs_preds b event;
+                admit();
 
                 // create and send fourth message
                 let msg4:message now = Msg4 c (|tag_ev_a,c_ev_a|) in
@@ -363,8 +390,6 @@ let responder_send_msg_4 b msg3_idx b_si =
                 includes_can_flow_lemma now [P b; P srv] [P b];
                 can_flow_transitive now (get_label oyrs_key_usages k_ab) (readers [P b; P srv]) (readers [P b]);
                 assert(is_msg oyrs_global_usage now k_ab (readers [P b]));
-                // prev -> now
-                assert(can_aead_encrypt prev "sk_r_srv" k_bs tagged_ser_ev_b ad ==> (exists p. was_rand_generated_before prev k_ab (readers [P srv; P p; P b]) (aead_usage "sk_i_r")));
                 let ser_st = serialize_session_st now b b_si b_vi st_r_sent_m4 in
                 update_session #oyrs_preds #now b b_si b_vi ser_st;
 
